lambda2Gmu/Equations.v
@@ -1,8 +1,5 @@
-Require Import TLC.LibLN.
-Require Import Definitions.
-Require Import TLC.LibTactics.
-Require Import List.
-Import List.ListNotations.
+Require Import Prelude.
+Require Import Infrastructure.
 
 (* Proofs regarding proposition 2.1 from the paper *)
 
@@ -37,3 +34,59 @@ Section SimpleEquationProperties.
   Qed.
 
 End SimpleEquationProperties.
+
+Lemma spawn_unit_subst : forall Σ As,
+    exists Θ, length Θ = length As /\ subst_matches_typctx Σ (tc_vars As) Θ.
+  induction As as [| Ah Ats].
+  - cbn.
+    exists (@nil (var * typ)).
+    split~.
+    constructor.
+  - destruct IHAts as [LT [Len Match]].
+    exists ((Ah, typ_unit) :: LT).
+    split.
+    + cbn. auto.
+    + constructor.
+      * constructor.
+      * fold (List.map tc_var Ats).
+        fold (tc_vars Ats).
+        trivial.
+Qed.
+
+Lemma only_vars_is_tc_vars : forall Δ,
+    (forall tc, List.In tc Δ -> exists A, tc = tc_var A) ->
+    exists As, Δ = tc_vars As.
+  induction Δ as [| [A | eq] Δt].
+  - cbn. intros. exists (@nil var). cbn. trivial.
+  - cbn. intro Hin.
+    lets* [Ats EQ]: IHΔt.
+    exists (A :: Ats). cbn.
+    fold (tc_vars Ats).
+    f_equal.
+    auto.
+  - cbn. intro Hin.
+    false~ Hin. congruence.
+Qed.
+
+Lemma only_vars_is_never_contradictory : forall Σ Δ,
+    (forall tc, List.In tc Δ -> exists A, tc = tc_var A) ->
+    ~ (contradictory_bounds Σ Δ).
+  intros.
+  intro HF.
+  unfold contradictory_bounds in HF.
+  lets F: HF typ_unit (typ_unit ** typ_unit).
+  unfold entails_semantic in F.
+  lets* [As AsEQ]: only_vars_is_tc_vars. subst.
+  lets [Θ [TLen TMatch]]: spawn_unit_subst Σ As.
+  assert (Contr: typ_unit = typ_unit ** typ_unit).
+  - unfold alpha_equivalent in F.
+    lets F2: F TMatch.
+    rewrite subst_ttΘ_fresh in F2.
+    + rewrite~ subst_ttΘ_fresh in F2.
+      cbn.
+      rewrite union_empty_r.
+      rewrite~ inter_empty_r.
+    + cbn.
+      rewrite~ inter_empty_r.
+  - false.
+Qed.
